HTTCC: Bind, fetch, some algebra on state
We succeed to entail high order state operations, but still cannot join
them, we need to get rid of the dependency that pre and post introduce.

HTTCC.v
@@ -13,25 +13,35 @@
 Set Universe Polymorphism.
 Set Printing All.
 
-(* some toy state: until we get full ssreflect support and can
-re-implement HTT's heap *)
+(* 
+** Some toy state: until we get full ssreflect support and can
+** re-implement HTT's heaps
+*)
 
-Parameter (heap : Type -> Type).
+Parameter (state : Type -> Type).
 
-Definition pre W := heap W -> Prop.
-Definition post W X := X -> heap W -> heap W -> Prop.
+(* Some algebra over  state *)
 
-Parameter write: forall W,  W -> heap W -> heap W.
-Parameter read: forall  W, heap W -> W.
+Definition pre W := state W -> Prop.
+Definition post W X := X -> state W -> state W -> Prop.
+
+Parameter write: forall W,  W -> state W -> state W.
+Parameter read: forall  W, state W -> W.
+
+Axiom read_write : forall W h w,  read W (write W w h) = w.  
+
+Axiom write_write : forall W h w v,  
+                      write W w (write W w h) = write W v (write W w h).  
+
+Axiom write_read: forall W h, write W (read W h) h = h.
 
 
 (* A polymorphic HTT + State + Continuation monad *)
 
 Polymorphic Definition SK {A X W: Type} 
             (P : pre W) (Q: post W A) : Type :=
-  forall s: heap W, P s -> 
+  forall s: state W, P s -> 
                   (forall x m, Q x s m -> X) -> X.
-
 
 Arguments SK {A} X {W} P Q .
 
@@ -50,8 +60,41 @@ Definition ret : SK R ret_P ret_s :=
   fun s p k => @k x s (retQ_refl s).
 
 End Ret.
-
 Arguments ret {X} W R x s _ _ .
+
+
+Section Bind.
+Variables (A B W R: Type).
+Variables (p1: pre W) (q1: post W A).
+Variables (p2 : A -> pre W) (q2 : A -> post W B).
+Variables (e1 : SK R p1 q1) (e2 : forall x, SK R (p2 x) (q2 x)).
+
+Definition bind_pre : pre W := 
+  fun i => 
+     p1 i /\ forall x m, q1 x i m -> (p2 x) m.
+
+Definition bind_post : post W B := 
+   fun y i m => exists x, exists h, 
+     q1 x i h /\ (q2 x) y h m.
+
+
+Lemma bindP1 h : bind_pre h -> p1 h.
+Proof. intro H; case H; auto. Qed. 
+
+Lemma bindP2 i x h : bind_pre i -> q1 x i h -> (p2 x) h.
+Proof. intros P Q; destruct P; apply H0; auto. Qed.
+ 
+Lemma bindQ i x h y m : 
+        q1 x i h -> (q2 x) y h m -> bind_post y i m.
+Proof. intros; exists x; exists h; auto. Qed.
+
+Definition bind : SK R bind_pre bind_post :=
+ fun i pf1 k => 
+          e1 i (bindP1 i pf1) 
+           (fun x h p2 => (e2 x) h (bindP2 i x h pf1 p2) 
+           (fun y m p3 => k y m (bindQ i x h y m p2 p3))).
+End Bind.
+Arguments bind {A B W R p1 q1 p2 q2} e1 e2 _ _ _ .
 
 Section Store.
 Variables (X R :Type) (x:X).
@@ -67,39 +110,71 @@ Polymorphic
 Definition store : SK R write_P write_Q :=
   fun s p k => k tt (write X x s) (writeQ s).
 End Store.
-
 Arguments store {X} R x _  _ _. 
 
-Definition rr1:= ret False nat (ret False nat 5).
+Section Fetch.
+Variables (X R :Type).
 
-(* not-using the heap lets you get away with murder *)
+Definition read_P : pre X := fun i => exists v j,  
+                                        i = write X v j.
+Definition read_Q  : post X X :=
+  fun r i m =>  forall v j, i = write X v j ->
+                  m = i /\ r = v.
 
-Definition st1:= store nat (ret nat nat 5). 
+Lemma fetchQ s :  read_Q (read X s) s s.
+Proof. intros v j H; split ;[|rewrite H ;rewrite (read_write X j)]; auto. Qed.
 
-Definition sst1 := store unit (st1).
+Polymorphic 
+Definition fetch : SK R read_P read_Q :=
+  fun s p k => k (read X s) s (fetchQ s).
+End Fetch.
+Arguments fetch {X R} _ _ _.
 
-Set Printing Universes.
 
-Check st1.
+(* Some examples *)
 
-Check sst1.
 
-(*  st1 = 
-@store (@SK nat nat N (ret_P N) (ret_s nat N (S (S (S (S (S O))))))) nat
-  (@ret nat N nat (S (S (S (S (S O))))))
-     : @SK unit nat
-         (@SK nat nat N (ret_P N) (ret_s nat N (S (S (S (S (S O)))))))
-         (write_P
-            (@SK nat nat N (ret_P N) (ret_s nat N (S (S (S (S (S O))))))))
-         (write_Q
-            (@SK nat nat N (ret_P N) (ret_s nat N (S (S (S (S (S O)))))))
-            (@ret nat N nat (S (S (S (S (S O)))))))
+Polymorphic 
+Definition rr1 {A: Type}
+  := ret A nat (ret A nat 5).
 
-st1 is universe polymorphic
+Polymorphic 
+Definition st1 {A B : Type} 
+            := store A (ret B unit 5). 
 
+Definition  br1 
+  := bind (store nat 4) 
+          (fun _ => bind fetch (ret _ _ )).
+
+Polymorphic Definition id {A : Type} (a : A) := a.
+
+(* I can Join rets *)
+
+Definition brr1 {A: Type} := bind (@rr1 A) id.
+
+(* However, I have to explicitly mention the state type here *)
+
+
+(* I can store a program and then read it *)
+Polymorphic 
+Definition bsf {A B: Type} := bind (@st1 A B) (fun _ => fetch).
+
+(* 
+** Can I flatten it straight away?  
+**    join : SK (SK A) -> SK A := fun m => bind m id
+**
 *)
 
 
+Fail Polymorphic 
+Definition bsf' := 
+    bind bsf id.
+
+(* 
+** Well, I guess that I  would still need 
+**   Sigma types for pulling something like this.
+** Or a  proper join. 
+*)
 
 
 
